src/MicroSail/Symbolic/Mutator.v
@@ -237,13 +237,13 @@ Module Mutators
     Equations(noeqns) match_chunk_eqb (ce : Chunk Σ) (cr : Chunk Σ) :
       PathCondition Σ -> option (PathCondition Σ) :=
       match_chunk_eqb (chunk_pred p1 ts1) (chunk_pred p2 ts2)
-      with 𝑷_eq_dec p1 p2 => {
+      with eq_dec p1 p2 => {
         match_chunk_eqb (chunk_pred p1 ts1) (chunk_pred p2 ts2) (left eq_refl) := match_env_eqb ts1 ts2;
-        match_chunk_eqb (chunk_pred p1 ts1) (chunk_pred p2 ts2) (right _) := fun _ => None
+        match_chunk_eqb (chunk_pred p1 ts1) (chunk_pred p2 ts2) (right _)      := fun _ => None
       };
       match_chunk_eqb (chunk_ptsreg r1 t1) (chunk_ptsreg r2 t2)
-      with 𝑹𝑬𝑮_eq_dec r1 r2 => {
-        match_chunk_eqb (chunk_ptsreg r1 t1) (chunk_ptsreg r2 t2) (left (@teq_refl eq_refl eq_refl)) := match_term_eqb t1 t2;
+      with eq_dec_het r1 r2 => {
+        match_chunk_eqb (chunk_ptsreg r1 t1) (chunk_ptsreg r2 t2) (left eq_refl) := match_term_eqb t1 t2;
         match_chunk_eqb (chunk_ptsreg r1 t1) (chunk_ptsreg r2 t2) (right _)      := fun _ => None
       };
       match_chunk_eqb _ _  := fun _ => None.
@@ -331,13 +331,13 @@ Module Mutators
     Equations(noeqns) match_chunk (ce : Chunk Σe) (cr : Chunk Σr) :
       EvarEnv Σe Σr -> option (EvarEnv Σe Σr) :=
       match_chunk (chunk_pred p1 ts1) (chunk_pred p2 ts2)
-      with 𝑷_eq_dec p1 p2 => {
+      with eq_dec p1 p2 => {
         match_chunk (chunk_pred p1 ts1) (chunk_pred p2 ts2) (left eq_refl) := match_env ts1 ts2;
-        match_chunk (chunk_pred p1 ts1) (chunk_pred p2 ts2) (right _) := fun _ => None
+        match_chunk (chunk_pred p1 ts1) (chunk_pred p2 ts2) (right _)      := fun _ => None
       };
       match_chunk (chunk_ptsreg r1 t1) (chunk_ptsreg r2 t2)
-      with 𝑹𝑬𝑮_eq_dec r1 r2 => {
-        match_chunk (chunk_ptsreg r1 t1) (chunk_ptsreg r2 t2) (left (@teq_refl eq_refl eq_refl)) := match_term t1 t2;
+      with eq_dec_het r1 r2 => {
+        match_chunk (chunk_ptsreg r1 t1) (chunk_ptsreg r2 t2) (left eq_refl) := match_term t1 t2;
         match_chunk (chunk_ptsreg r1 t1) (chunk_ptsreg r2 t2) (right _)      := fun _ => None
       };
       match_chunk _ _  := fun _ => None.
